GMLInit/Data/HList.lean
@@ -1,12 +1,41 @@
 import GMLInit.Data.Basic
 import GMLInit.Data.HVal
+import GMLInit.Logic.Eq
+import GMLInit.Logic.ListConnectives
 import GMLInit.Meta.Basic
+import GMLInit.Meta.Relation
 
 inductive HList.{u} : List (Sort u) → Type u
 | nil : HList []
 | cons {α αs} : α → HList αs → HList (α :: αs)
 
 namespace HList
+
+protected def extAux : {αs βs : List (Sort _)} → (as : HList αs) → (bs : HList βs) → List Prop
+| [], [], nil, nil => []
+| [], _::_, nil, cons _ _ => [False]
+| _::_, [], cons _ _ , nil => [False]
+| _::_, _::_, cons a as, cons b bs => (a ≅ b) :: HList.extAux as bs
+
+protected theorem ext {αs : List (Sort _)} (as₁ as₂ : HList αs) : All (HList.extAux as₁ as₂) → as₁ = as₂ := by
+  intro h
+  induction as₁ with
+  | nil =>
+    cases as₂ with
+    | nil => rfl
+  | cons a₁ as₁ H =>
+    cases as₂ with
+    | cons a₂ as₂ =>
+      cases h with
+      | cons h hs =>
+        rw [eq_of_heq h, H _ hs]
+
+protected theorem dext {αs βs : List (Sort _)} (as : HList αs) (bs : HList βs) : αs = βs → All (HList.extAux as bs) → as ≅ bs := by
+  intro ht hs
+  cases ht
+  apply heq_of_eq
+  apply HList.ext
+  exact hs
 
 protected def mk : {αs : List (Sort _)} → ((i : Index αs) → i.val) → HList αs
 | [], _ => nil
@@ -31,18 +60,19 @@ def eval : {αs : List (Sort _)} → HList αs → (i : Index αs) → i.val
 def equiv (αs : List (Sort _)) : Equiv (HList αs) ((i : Index αs) → i.val) where
   fwd := HList.eval
   rev := HList.mk
-  spec as vs := by
+  spec := by
+    intros as f
     constr
     · intro h
       cases h
       induction as with
       | nil => rfl
-      | cons a as H => simp only [HList.mk, HList.eval, H]
+      | cons a as H => unfold HList.mk HList.eval; rw [H]
     · intro h
       cases h
       funext i
       induction i with
       | head => rfl
-      | tail i H => simp only [HList.eval, HList.mk, H]
+      | tail i H => unfold HList.eval HList.mk; rw [H]
 
 end HList
