GMLInit/Data/Option.lean
@@ -11,12 +11,12 @@ namespace Option
 @[simp] lemma id_map {α} (a : Option α) : a.map id = a := by
   cases a with
   | none => rfl
-  | some _ => rfl
+  | some => rfl
 
-lemma comp_map {α β γ} (g : β → γ) (f : α → β) (a : Option α) : (a.map f).map g = a.map (g ∘ f) := by
+lemma comp_map {α β γ} (g : β → γ) (f : α → β) (a : Option α) : a.map (g ∘ f) = (a.map f).map g := by
   cases a with
   | none => rfl
-  | some _ => rfl
+  | some => rfl
 
 @[simp] lemma none_bind {α β} (f : α → Option β) : none.bind f = none := rfl
 
@@ -25,18 +25,19 @@ lemma comp_map {α β γ} (g : β → γ) (f : α → β) (a : Option α) : (a.m
 lemma bind_assoc {α β γ} (f : α → Option β) (g : β → Option γ) (a : Option α) : (a.bind f).bind g = a.bind (λ a => (f a).bind g) := by
   cases a with
   | none => rfl
-  | some _ => rfl
+  | some => rfl
 
 def equiv {α β} (e : Equiv α β) : Equiv (Option α) (Option β) where
   fwd := Option.map e.fwd
   rev := Option.map e.rev
-  spec a b := by
+  spec := by
+    intros
     constr
     · intro h
       cases h
-      rw [comp_map, e.comp_rev_fwd, id_map]
+      rw [←comp_map, e.comp_rev_fwd, id_map]
     · intro h
       cases h
-      rw [comp_map, e.comp_fwd_rev, id_map]
+      rw [←comp_map, e.comp_fwd_rev, id_map]
 
 end Option
